Test/Assumption.lean
@@ -1,0 +1,53 @@
+import Veil
+
+veil module Blockchain
+
+type node
+type block
+type transaction
+type time
+
+instantiate tot : TotalOrder time
+
+immutable relation leader : node → time → Prop
+
+relation honest : node → Prop
+relation broadcastable : node → block → time → Prop
+relation broadcasted : node → Prop
+
+relation block_found : node → block → time → Prop
+relation block_confirmed : node → block → time → Prop
+
+immutable relation transaction_time : transaction → time → Prop
+
+relation transaction_in_block : transaction → block → Prop
+relation transaction_confirmed : transaction → node → Prop
+
+#gen_state
+
+assumption leader N1 T ∧ leader N2 T → N1 = N2
+assumption leader N T1 ∧ leader N T2 → T1 = T2
+
+after_init {
+    block_found N B T := False;
+    block_confirmed N B T := False;
+    transaction_in_block TR B := False;
+    transaction_confirmed TR N := False;
+    broadcasted N := False;
+    broadcastable N B T := False
+}
+
+/-- error: All assumptions must be defined before the after_init declaration! -/
+#guard_msgs in
+assumption transaction_time TR T1 ∧ transaction_time TR T2 → T1 = T2
+
+action find_block (n : node) (b : block) (t: time) = {
+  require leader n t;
+  block_found n b t := True
+}
+
+invariant True
+
+#gen_spec
+
+end Blockchain
